working on basic math constructions

Math/sorting/ordering.v
@@ -1,14 +1,5 @@
-Inductive natlist : Type :=
-  | nil : natlist
-  | cons : nat -> natlist -> natlist.
-
-Axiom nat_default : nat.
-
-Fixpoint head (l : natlist) :=
-  match l with
-  | nil => nat_default
-  | cons h t => h
-  end.
+Add LoadPath "/Users/Henry/Documents/Drive/Coq/Math/sorting".
+Load natlist.
 
 Fixpoint eqb (n m : nat) :=
   match n,m with
@@ -27,20 +18,49 @@ Fixpoint leb (n m : nat) :=
 
 Definition can_head (n : nat) (l : natlist) :=
   match l with
-  | nil => true
-  | cons m _ => leb n m
+  | []   => true
+  | m::_ => leb n m
   end.
 
 Inductive sorted : natlist -> Prop :=
-  | sorted_nil  : sorted nil
+  | sorted_nil  : sorted []
   | sorted_cons : forall (n : nat) (l : natlist),
       sorted l -> can_head n l = true -> sorted (cons n l).
 
-Example singleton_is_sorted : forall n, sorted (cons n nil).
+Example sorted_singleton : forall n, sorted (cons n nil).
 Proof.
   intros.
   refine (sorted_cons _ _ _ _ ).
   apply sorted_nil.
-  exact (eq_refl : can_head n nil = true).
+  exact (eq_refl : can_head n [] = true).
 Qed.
 
+Ltac red_sorted_cons := (refine (sorted_cons _ _ _ _)).
+
+(* Example example1 : sorted (cons 1 (cons 2 (cons 3 nil))). *)
+Example sorted_example1 : sorted [1;2;3].
+Proof.
+  red_sorted_cons. red_sorted_cons. red_sorted_cons.
+  apply sorted_nil.
+  apply eq_refl. apply eq_refl. apply eq_refl.
+Qed.
+
+Example sorted_example2 : ~ sorted [2;1].
+Proof.
+  unfold not.
+  intros.
+  inversion H.
+  simpl in H3.
+  discriminate.
+Qed.
+
+Example sorted_example3 : forall n, sorted [n;S n].
+Proof.
+  intros. red_sorted_cons. red_sorted_cons.
+  apply sorted_nil.
+  simpl. reflexivity.
+  simpl. cut (leb n (S n) = true). intros. exact H.
+  induction n.
+    simpl. reflexivity.
+    simpl. apply IHn.
+Qed.
