Math/combinatorics/pascal.v
@@ -1,0 +1,77 @@
+Notation Nat := nat.
+
+Fixpoint factorial (n:Nat) : Nat :=
+  match n with
+  | O   => 1
+  | S n => (S n) * factorial n
+  end.
+
+Fixpoint eq_nat (n m:Nat) : bool :=
+  match n,m with
+  | O  ,O   => true
+  | S _,O   => false
+  | O  ,S _ => false
+  | S o,S p => eq_nat o p
+  end.
+
+Fixpoint subtract (n m:Nat) : Nat :=
+  match n,m with
+  | O  ,_   => O
+  | S _,O   => n
+  | S o,S p => subtract o p
+  end.
+
+Inductive Fraction : Set :=
+  | frac : forall (n d:Nat), d <> O -> Fraction.
+
+Lemma add_id_right : forall n, n + O = n.
+Proof.
+  intro n.
+  induction n.
+  simpl. reflexivity.
+  simpl. rewrite IHn. reflexivity.
+Qed.
+
+Lemma succ_gt_O : forall n, S n > O.
+Proof.
+  intro n.
+  induction n.
+  auto.
+  auto.
+Qed.
+
+Lemma factorial_gt_O : forall (n:Nat), factorial n > O.
+Proof. Admitted.
+
+Lemma product_preserves_gt_O :
+  forall (n m:Nat), n > O -> m > O -> n * m > O.
+Proof. Admitted.
+
+Lemma gt_O_implies_neq_O : forall n, n > O -> n <> O.
+Proof.
+  intros n n_gt_O.
+  unfold not. intro n_eq_O.
+  destruct n_gt_O.
+  discriminate.
+  discriminate.
+Qed.
+
+Definition binomial (n k:Nat) : Fraction.
+  refine (frac _ _ _).
+  exact (factorial n).
+  pose (d := ((factorial (subtract n k)) * (factorial k))).
+  cut (d > O). intro d_gt_O.
+  apply gt_O_implies_neq_O in d_gt_O.
+  apply d_gt_O.
+  apply product_preserves_gt_O.
+  apply factorial_gt_O.
+  apply factorial_gt_O.
+Qed.
+
+Compute (binomial 2 1).
+
+Lemma one_neq_O : 1 <> O. Proof. Admitted.
+
+Lemma x : forall n m, binomial n m = frac 1 1 one_neq_O.
+  intros.
+  simpl. 
