Math/geometry/euclid.v
@@ -1,0 +1,53 @@
+(*–––––––––––––––––––––––––––––––––––+
+ |
+ |  Euclid's Axioms for Geometry
+ |
+ +–––––––––––––––––––––––––––––––––––*)
+
+
+(* Basic Types *)
+Axiom Point : Set.
+
+(* Axiom 1 *)
+Inductive Segment : Set :=
+  segment_from_points : Point -> Point -> Segment.
+
+(* Axiom 2 *)
+Inductive Line : Set :=
+  line_from_segment : Segment -> Line.
+
+(* Axiom 3 *)
+Inductive Circle : Set :=
+  circle_from_points : Point -> Point -> Circle.
+
+(* Axiom 4 *)
+Axiom Angle : Set.
+Axiom angle_between : Line -> Line -> Angle.
+Axiom right : Angle.
+
+Axiom lines_angles_equality:
+  forall l l' l'' : Line,
+  angle_between l l'  = angle_between l l''
+  -> l' = l''.
+
+Proposition lines_right_angles_equality:
+  forall l l' l'',
+  angle_between l l'  = right
+  -> angle_between l l'' = right
+  -> l' = l''.
+Proof.
+  intros.
+  cut (angle_between l l' = angle_between l l''). intro.
+  apply (lines_angles_equality l l' l'' H1).
+  pose (H1 := eq_sym H0).
+  apply (eq_trans H H1).
+Qed.
+
+Inductive right_angled : Line -> Line -> Prop :=
+  right_lines : forall l l', angle_between l l' = right -> right_angled l l'.
+
+(* Axiom 5 *)
+Axiom nonperpendicular_lines_intersect:
+  forall l l',
+  ~ right_angled l l' 
+
