Math/sorting/example_bubblesort.v
@@ -1,0 +1,55 @@
+Require Import List.
+Require Import Arith.
+Require Import Sorted.
+Require Import Recdef.
+
+Function bubble (l : list nat) {measure length} : list nat :=
+  match l with
+  | nil => nil
+  | n :: nil => n :: nil
+  | n1 :: n2 :: l' => if leb n1 n2
+                      then n1 :: (bubble (n2 :: l'))
+                      else n2 :: (bubble (n1 :: l'))
+  end.
+Proof.
+  auto. auto.
+Qed.
+
+Function bubble_sort (l : list nat) : list nat :=
+  match l with
+  | nil => nil
+  | n :: l' => bubble (n :: (bubble_sort l'))
+  end.
+
+Check Sorted.
+
+Check (Sorted le).
+
+Print Sorted.
+
+Print HdRel.
+
+(* 
+Sorted_cons:
+  forall (a : A) (l : list A),
+  Sorted R l -> HdRel R a l -> Sorted R (a :: l)
+
+HdRel_nil : HdRel R a nil
+HdRel_cons : forall (b : A) (l : list A), R a b -> HdRel R a (b :: l)
+*)
+
+Check bubble_terminate.
+Check iter.
+
+Theorem bubble_sort_correct : forall l, Sorted le (bubble_sort l).
+Proof.
+  intros.
+  induction l.
+    simpl. apply Sorted_nil.
+    simpl. destruct l.
+      simpl. unfold bubble.
+      unfold bubble_terminate.
+
+Eval compute in bubble      (1 :: 2 :: 0 :: 3 :: 1 :: nil).
+Eval compute in bubble_sort (1 :: 2 :: 0 :: 3 :: 1 :: nil).
+Eval compute in bubble_sort (1 :: 2 :: 10 :: 3 :: 6 :: nil).
