Math/sorting/example_bublesort01.v
@@ -1,0 +1,43 @@
+Require Import List.
+Require Import Arith.
+Require Import Sorted.
+Require Import Recdef.
+
+Function bubble (l : list nat) {measure length} : list nat :=
+  match l with
+  | nil      => nil
+  | n::nil   => n::nil
+  | n::m::l' =>
+      if leb n m
+        then n::( bubble (m::l') )
+        else m::( bubble (n::l') )
+  end.
+Proof. auto. auto. Qed.
+
+Search lt.
+
+Function bubble (l : list nat) {measure length} : list nat :=
+  match l with
+  | nil => nil
+  | n :: nil => n :: nil
+  | n1 :: n2 :: l' => if leb n1 n2
+                      then n1 :: (bubble (n2 :: l'))
+                      else n2 :: (bubble (n1 :: l'))
+  end.
+Proof.
+  auto. auto.
+Qed.
+
+Function bubble_sort (l : list nat) : list nat :=
+  match l with
+  | nil => nil
+  | n :: l' => bubble (n :: (bubble_sort l'))
+  end.
+
+
+  | n::nil   => n::nil
+  | n::m::l' =>
+      if leb n m
+        then n::( bubble (m::l') )
+        else m::( bubble (n::l') )
+  end.
