Math/sorting/natlist.v
@@ -1,0 +1,49 @@
+Inductive natlist : Type :=
+  | nil : natlist
+  | cons : nat -> natlist -> natlist.
+
+Notation "[ ]" := nil (format "[ ]").
+Notation "[ x ]" := (cons x nil).
+Notation "[ x ; y ; .. ; z ]" := (cons x (cons y .. (cons z nil) ..)).
+Notation "h :: t" := (cons h t) (at level 60, right associativity).
+
+Axiom nat_default : nat.
+
+Definition head (l : natlist) :=
+  match l with
+  | []   => nat_default
+  | h::t => h
+  end.
+
+Definition head_safe (l : natlist) (safety : ~ l = nil) : nat.
+  destruct l.
+  unfold not in safety.
+  case (safety (eq_refl : [] = [])).
+  exact n.
+Defined.
+
+Lemma not_nil_example1 : ~ [1;2] = nil.
+Proof. intros. unfold not. intros. inversion H. Qed.
+
+Example head_safe_example1 : head_safe [1;2] not_nil_example1 = 1.
+Proof. simpl. reflexivity. Qed.
+
+Fixpoint append (n : nat) (l : natlist) : natlist :=
+  match l with
+  | [] => [n]
+  | h::t => h :: (append n t)
+  end.
+
+Fixpoint concat (xs ys : natlist) : natlist :=
+  match ys with
+  | [] => ys
+  | h::t => concat (append h xs) t
+  end.
+
+Notation "xs ++ ys" := (concat xs ys) (at level 60, right associativity).
+
+Fixpoint length (l : natlist) :=
+  match l with
+  | [] => 0
+  | _::t => 1 + length t
+  end.
