Math/sorting/sorting.v
@@ -1,0 +1,53 @@
+Add LoadPath "/Users/Henry/Documents/Drive/Coq/Math/sorting".
+Load ordering.
+
+Fixpoint removelast (l : natlist) :=
+  match l with
+  | []    => []
+  | h::[] => []
+  | h::t  => h :: removelast t
+  end.
+
+Fixpoint last (l : natlist) (default : nat) :=
+  match l with
+  | []    => default
+  | h::[] => h
+  | h::t  => last t default
+  end.
+
+Fixpoint bubble_sort' (l : natlist) (n : nat) (time : nat) : natlist :=
+  match time with
+  | 0    => l
+  | S t' =>
+      match l with
+      | nil => nil
+      | cons n' nil =>
+          match (leb n n') with
+          | true  => cons n  (cons n' nil)
+          | false => cons n' (cons n nil)
+          end
+      | cons n' (cons n'' _ as l') =>
+          match (leb n n') with
+          | true  => let l'' :=
+              bubble_sort' l' n' t' in
+              (bubble_sort' (removelast l'') n  t') ++ ((last l'' 0) :: nil)
+          | false => let l'' :=
+              bubble_sort' l' n  t' in
+              (bubble_sort' (removelast l'') n' t') ++ ((last l'' 0) :: nil)
+          end
+      end
+  end.
+
+Fixpoint bubble_sort (l : natlist) : natlist :=
+  match l with
+  | nil => nil
+  | h::[] => h::[]
+  | h::t  => bubble_sort' t h (length t)
+  end.
+
+Compute (bubble_sort [2;1]).
+
+Check measure.
+
+Eval compute in .
+Eval compute in bubble_sort (1 :: 2 :: 10 :: 3 :: 6 :: nil).
